code/ed25519/Hacl.Impl.Ed25519.Verify.fst
@@ -12,7 +12,6 @@ open Lib.Buffer
 open Hacl.Bignum25519
 
 module F51 = Hacl.Impl.Ed25519.Field51
-module F56 = Hacl.Impl.Ed25519.Field56
 
 #reset-options "--z3rlimit 20 --max_fuel 0 --max_ifuel 0"
 
